more

thys/Substitution/Expression_Like_Birecursor.thy
@@ -7,15 +7,26 @@ locale Bimodel = Nominal Pperm "PVrs :: 'p \<Rightarrow> 'a :: var set" + Expres
   fixes  is_base :: "('a::var, 'a, 'e, 'e) G \<Rightarrow> bool"
   and Ector_base :: "('a::var, 'a, 'e, 'e) G \<Rightarrow> 'p \<Rightarrow> 'e"
   and Ector_step :: "('a::var, 'a, 'p \<Rightarrow> 'e, 'p \<Rightarrow> 'e) G \<Rightarrow> 'p \<Rightarrow> 'e"
-  assumes TODO: "\<exists>P. P is_base Ector_base Ector_step"
+  assumes TODO: "\<exists>P. P is_base Ector_base Ector_step" (* TODO 1 here we need the assumptions on bimodels*)
 
-locale Birecursor = Bimodel Pperm "PVrs :: 'p \<Rightarrow> 'a set" Eperm "EVrs :: 'e \<Rightarrow> 'a :: var set" Ector is_base Ector_base Ector_step
-  for Pperm PVrs Eperm EVrs Ector is_base Ector_base Ector_step +
-  assumes rec: "\<exists>rec.
+(*
+TODO the below Birecursor locale needs to be interpreted for both datatypes and codatatypes
+in the respective theory Data and Codata using the recursor/corecursor
+the existing interpretations in that theory that define substitution directly should be quite close
+*)
+locale Birecursor = Expression Eperm "EVrs :: 'e \<Rightarrow> 'a :: var set" Ector
+  for Eperm EVrs Ector +
+  fixes Pdummy :: 'p
+  assumes rec: "\<forall>Pperm (PVrs :: 'p \<Rightarrow> 'a set) is_base Ector_base Ector_step.
+    Bimodel Pperm PVrs Eperm EVrs Ector is_base Ector_base Ector_step \<longrightarrow> (\<exists>rec.
       ((\<forall>u p. is_base u \<longrightarrow> GVrs2 u \<inter> PVrs p = {} \<longrightarrow> rec (Ector u) p = Ector_base u p) \<and>
        (\<forall>u p. \<not> is_base u \<longrightarrow> GVrs2 u \<inter> PVrs p = {} \<longrightarrow> rec (Ector u) p = Ector_step (Gmap rec rec u) p) \<and>
        (\<forall>e p \<sigma>. bij \<sigma> \<longrightarrow> |supp \<sigma>| <o |UNIV :: 'a set| \<longrightarrow> rec (Eperm \<sigma> e) p = Eperm \<sigma> (rec e (Pperm (inv \<sigma>) p))) \<and>
-       (\<forall>e p. EVrs (rec e p) \<subseteq> PVrs p \<union> EVrs e))"
+       (\<forall>e p. EVrs (rec e p) \<subseteq> PVrs p \<union> EVrs e)))"
+begin
+
+context fixes Pperm and PVrs :: "'p \<Rightarrow> 'a set" and is_base Ector_base Ector_step
+  assumes BM: "Bimodel Pperm PVrs Eperm EVrs Ector is_base Ector_base Ector_step"
 begin
 
 definition rec where
@@ -25,20 +36,22 @@ definition rec where
        (\<forall>e p. EVrs (rec e p) \<subseteq> PVrs p \<union> EVrs e)))"
 
 lemma rec_base: "is_base u \<Longrightarrow> GVrs2 u \<inter> PVrs p = {} \<Longrightarrow> rec (Ector u) p = Ector_base u p"
-  using someI_ex[OF rec, THEN conjunct1] unfolding rec_def
+  using someI_ex[OF rec[rule_format, OF BM], THEN conjunct1] unfolding rec_def
   by blast
 
 lemma rec_Ector: "\<not> is_base u \<Longrightarrow> GVrs2 u \<inter> PVrs p = {} \<Longrightarrow> rec (Ector u) p = Ector_step (Gmap rec rec u) p"
-  using someI_ex[OF rec, THEN conjunct2, THEN conjunct1] unfolding rec_def
+  using someI_ex[OF rec[rule_format, OF BM], THEN conjunct2, THEN conjunct1] unfolding rec_def
   by blast
 
 lemma rec_EPerm: "bij \<sigma> \<Longrightarrow> |supp \<sigma>| <o |UNIV :: 'a set| \<Longrightarrow> rec (Eperm \<sigma> e) p = Eperm \<sigma> (rec e (Pperm (inv \<sigma>) p))"
-  using someI_ex[OF rec, THEN conjunct2, THEN conjunct2, THEN conjunct1] unfolding rec_def
+  using someI_ex[OF rec[rule_format, OF BM], THEN conjunct2, THEN conjunct2, THEN conjunct1] unfolding rec_def
   by blast
 
 lemma rec_EVrs: "EVrs (rec e p) \<subseteq> PVrs p \<union> EVrs e"
-  using someI_ex[OF rec, THEN conjunct2, THEN conjunct2, THEN conjunct2] unfolding rec_def
+  using someI_ex[OF rec[rule_format, OF BM], THEN conjunct2, THEN conjunct2, THEN conjunct2] unfolding rec_def
   by blast
+
+end
 
 end
 
@@ -78,16 +91,24 @@ lemma permute_\<rho>':
    apply (auto simp: IImsupp'_def IImsupp_def SSupp_def imsupp_def supp_def)
   done
 
-sublocale Esub: Birecursor where
-  Pperm = "\<lambda>\<sigma> (\<delta>, \<rho>, \<rho>'). (\<sigma> o \<delta> o inv \<sigma>, Eperm \<sigma> o \<rho> o inv \<sigma>, Eperm \<sigma> o \<rho>' o inv \<sigma>)" and
-  PVrs = "\<lambda>(\<delta>, \<rho>, \<rho>'). imsupp \<delta> \<union> IImsupp' (Ector \<circ> \<eta>) EVrs \<rho> \<union> IImsupp' (Ector \<circ> \<eta>') EVrs \<rho>'" and
+definition "Esub_Pperm \<equiv> \<lambda>\<sigma> (\<delta>, \<rho>, \<rho>'). (\<sigma> o \<delta> o inv \<sigma>, Eperm \<sigma> o \<rho> o inv \<sigma>, Eperm \<sigma> o \<rho>' o inv \<sigma>)"
+definition "Esub_PVrs \<equiv> \<lambda>(\<delta>, \<rho>, \<rho>'). imsupp \<delta> \<union> IImsupp' (Ector \<circ> \<eta>) EVrs \<rho> \<union> IImsupp' (Ector \<circ> \<eta>') EVrs \<rho>'"
+definition "Esub_is_base \<equiv> \<lambda>u. \<exists>a. u = \<eta> a \<or> u = \<eta>' a"
+definition "Esub_Ector_base \<equiv> \<lambda>u (\<delta>, \<rho>, \<rho>'). if (\<exists>a. u = \<eta> a) then \<rho> (SOME a. u = \<eta> a) else \<rho>' (SOME a. u = \<eta>' a)"
+definition "Esub_Ector_step \<equiv> \<lambda>u (\<delta>, \<rho>, \<rho>'). Ector (Gsub \<delta> id (Gmap (\<lambda>rec. rec (\<delta>, \<rho>, \<rho>')) (\<lambda>rec. rec (\<delta>, \<rho>, \<rho>')) u))"
+lemmas Esub_defs = Esub_Pperm_def Esub_PVrs_def Esub_is_base_def Esub_Ector_base_def Esub_Ector_step_def
+
+sublocale Esub: Bimodel where
+  Pperm = Esub_Pperm and
+  PVrs = Esub_PVrs and
   Eperm = Eperm and
   EVrs = EVrs and
   Ector = Ector and
-  is_base = "\<lambda>u. \<exists>a. u = \<eta> a \<or> u = \<eta>' a" and
-  Ector_base = "\<lambda>u (\<delta>, \<rho>, \<rho>'). if (\<exists>a. u = \<eta> a) then \<rho> (SOME a. u = \<eta> a) else \<rho>' (SOME a. u = \<eta>' a)" and
-  Ector_step = "\<lambda>u (\<delta>, \<rho>, \<rho>'). Ector (Gsub \<delta> id (Gmap (\<lambda>rec. rec (\<delta>, \<rho>, \<rho>')) (\<lambda>rec. rec (\<delta>, \<rho>, \<rho>')) u))"
+  is_base = Esub_is_base and
+  Ector_base = Esub_Ector_base and
+  Ector_step = Esub_Ector_step
   apply standard
+  apply (unfold Esub_defs)
   subgoal for \<sigma> \<tau>
     by (auto simp: fun_eq_iff o_inv_distrib Eperm_comp[THEN fun_cong, simplified])
   subgoal for \<sigma> p
@@ -98,22 +119,31 @@ sublocale Esub: Birecursor where
     apply (metis (no_types, lifting) Int_emptyI bij_id_imsupp inv_simp2 permute_\<rho>')
     done
   subgoal
-    sorry
-  subgoal
+    (*trivial for now but needs a proper proof once the Bimodel properties are there*)
     sorry
   done
 
-definition "Esub \<delta> \<rho> \<rho>' e = Esub.rec e (\<delta>, \<rho>, \<rho>')"
+end
 
-interpretation Substitution Eperm EVrs Ector Esub
+(*TODO after the Birecursor instance is there interpret this locale to get the Substitution and 
+its properties for free*)
+locale Birecursor_Sub = Birecursor where
+  Eperm = Eperm and EVrs = "EVrs :: 'e \<Rightarrow> 'a :: var set" and Ector = Ector and
+  Pdummy = "undefined :: ('a \<Rightarrow> 'a) \<times> ('a \<Rightarrow> 'e)  \<times> ('a \<Rightarrow> 'e)"
+  for Eperm EVrs Ector
+begin
+
+definition "Esub \<delta> \<rho> \<rho>' e = rec Esub_Pperm Esub_PVrs Esub_is_base Esub_Ector_base Esub_Ector_step e (\<delta>, \<rho>, \<rho>')"
+
+sublocale Esub: Substitution Eperm EVrs Ector Esub
   apply standard
       apply (unfold Esub_def)
-      apply (subst Esub.rec_base; auto simp add: eta_inject)
-      apply (subst Esub.rec_base; auto simp add: eta_distinct' eta'_inject)
-    apply (subst Esub.rec_Ector; auto simp add: G.Map_comp[THEN fun_cong, simplified] comp_def[of _ Esub.rec])
-   apply (rule order_trans[OF Esub.rec_EVrs]; simp)
-  apply (subst Esub.rec_EPerm; simp)
-  apply (rule arg_cong[where f = "\<lambda>p. Eperm _ (Esub.rec _ p)"])
+      apply (subst rec_base[OF Esub.Bimodel_axioms]; auto simp add: eta_inject Esub_defs)
+      apply (subst rec_base[OF Esub.Bimodel_axioms]; auto simp add: eta_distinct' eta'_inject Esub_defs)
+    apply (subst rec_Ector[OF Esub.Bimodel_axioms]; auto simp add: G.Map_comp[THEN fun_cong, simplified] comp_def Esub_defs)
+   apply (rule order_trans[OF rec_EVrs[OF Esub.Bimodel_axioms]]; simp add: Esub_defs)
+  apply (subst rec_EPerm[OF Esub.Bimodel_axioms]; simp add: Esub_defs)
+  apply (rule arg_cong[where f = "\<lambda>p. Eperm _ (rec _ _ _ _ _ _ p)"])
   apply (auto simp: fun_eq_iff)
   apply (metis Int_Un_empty Int_emptyD bij_inv_rev imsupp_idle2 not_in_imsupp_same)
   apply (metis (mono_tags, lifting) Int_Un_empty Int_Un_emptyI1 bij_betw_inv_into imsupp_inv inv_simp1
@@ -125,3 +155,4 @@ interpretation Substitution Eperm EVrs Ector Esub
 end
 
 end
+
