thys/Substitution/Data.thy
@@ -124,16 +124,8 @@ interpretation Expression_Strong Eperm EVrs Ector Gbd
     done
   done
 
-context
-  fixes \<delta> :: "'a \<Rightarrow> 'a :: var_E_pre" and \<rho> \<rho>' :: "'a ::var_E_pre \<Rightarrow> 'a E"
-  assumes small_support:
-    "|supp (\<delta> :: 'a \<Rightarrow> 'a :: var_E_pre)| <o |UNIV::'a set|"
-    "|SSupp (Ector o \<eta>) (\<rho>::'a::var_E_pre \<Rightarrow> 'a E)| <o |UNIV::'a set|"
-    "|SSupp (Ector o \<eta>') (\<rho>'::'a::var_E_pre \<Rightarrow> 'a E)| <o |UNIV::'a set|"
-begin
-
 lemma permute_\<rho>:
-  "bij f \<Longrightarrow> |supp f| <o |UNIV :: 'a set| \<Longrightarrow> imsupp f \<inter> IImsupp' (Ector \<circ> \<eta>) EVrs \<rho> = {} \<Longrightarrow> Eperm f (\<rho> a) = \<rho> (f a)"
+  "bij f \<Longrightarrow> |supp (f :: 'a :: var_E_pre \<Rightarrow> 'a)| <o |UNIV :: 'a set| \<Longrightarrow> imsupp f \<inter> IImsupp' (Ector \<circ> \<eta>) EVrs \<rho> = {} \<Longrightarrow> Eperm f (\<rho> a) = \<rho> (f a)"
   apply (cases "f a = a")
    apply (cases "\<rho> a = Ector (\<eta> a)")
     apply (simp add: GMAP_def Gren_def eta_natural)
@@ -150,7 +142,7 @@ lemma permute_\<rho>:
   done
 
 lemma permute_\<rho>':
-  "bij f \<Longrightarrow> |supp f| <o |UNIV :: 'a set| \<Longrightarrow> imsupp f \<inter> IImsupp' (Ector \<circ> \<eta>') EVrs \<rho>' = {} \<Longrightarrow> Eperm f (\<rho>' a) = \<rho>' (f a)"
+  "bij f \<Longrightarrow> |supp (f :: 'a :: var_E_pre \<Rightarrow> 'a)| <o |UNIV :: 'a set| \<Longrightarrow> imsupp f \<inter> IImsupp' (Ector \<circ> \<eta>') EVrs \<rho>' = {} \<Longrightarrow> Eperm f (\<rho>' a) = \<rho>' (f a)"
   apply (cases "f a = a")
    apply (cases "\<rho>' a = Ector (\<eta>' a)")
     apply (simp add: GMAP_def Gren_def eta'_natural)
@@ -165,6 +157,14 @@ lemma permute_\<rho>':
    apply (simp add: GMAP_def Gren_def eta'_natural)
    apply (auto simp: IImsupp'_def IImsupp_def SSupp_def imsupp_def supp_def)
   done
+
+context
+  fixes \<delta> :: "'a \<Rightarrow> 'a :: var_E_pre" and \<rho> \<rho>' :: "'a ::var_E_pre \<Rightarrow> 'a E"
+  assumes small_support:
+    "|supp (\<delta> :: 'a \<Rightarrow> 'a :: var_E_pre)| <o |UNIV::'a set|"
+    "|SSupp (Ector o \<eta>) (\<rho>::'a::var_E_pre \<Rightarrow> 'a E)| <o |UNIV::'a set|"
+    "|SSupp (Ector o \<eta>') (\<rho>'::'a::var_E_pre \<Rightarrow> 'a E)| <o |UNIV::'a set|"
+begin
 
 interpretation Esub: QREC_fixed_E "imsupp \<delta> \<union> IImsupp' (Ector o \<eta>) EVrs \<rho> \<union> IImsupp' (Ector o \<eta>') EVrs \<rho>'"
   "\<lambda>u. if \<exists>a. Rep_E_pre u = \<eta> a then \<rho> (SOME a. Rep_E_pre u = \<eta> a) else
